Revert working file with DM

newio/DM.fst
@@ -66,167 +66,76 @@ let rec lemma_theta_is_monad_morphism_bind (m:io 'a) (f:'a -> io 'b) :
       == hist_bind (theta m) (fun x -> theta (f x))) by (rewrite_eqs_from_context ())
 
 // The Dijkstra Monad
-let dm (a:Type) (wp:hist a) (q:pure_post a) = 
-  m:(io (v:a{q v})){wp `hist_ord` theta m}
+let dm (a:Type) (wp:hist a) =
+  (m:(io a){wp `hist_ord` theta m})
 
-unfold
-let return_post (#a:Type) (x:a) : pure_post a = fun r -> r == x
-
-let dm_return (a : Type) (x : a) : dm a (hist_return x) (return_post x) =
+let dm_return (a : Type) (x : a) : dm a (hist_return x) =
   io_return x
 
-unfold
-let bind_post (#a #b:Type) (q1:pure_post a) (q2:a -> pure_post b) : pure_post b
-  = fun y -> exists x. q1 x ==> q2 x y
-
-let dm_subcomp
-  (q1 q2:pure_post 'a)
-  (wp1 wp2 : hist 'a)
-  (m: dm 'a wp1 q1) 
-  (_:squash (forall x. q1 x ==> q2 x))
-  (_:squash (wp1 `hist_ord` wp2)) :
-  dm 'a wp2 q2= 
-  admit ();
-  m
-
-let lemma_hist_monotonic
-  (a b : Type)
-  (wp_v : hist a)
-  (wp_f:  a -> hist b)
-  (post_v: pure_post a)
-  (post_f: a -> pure_post b)
-  (v : dm a wp_v post_v)
-  (f : (x:a{post_v x} -> dm b (wp_f x) (bind_post post_v post_f))) :
-  Lemma (
-  	hist_bind wp_v wp_f `hist_ord #(v:b{bind_post post_v post_f v})` 
-		  hist_bind (theta v) (fun x -> theta (f x)))
-  = admit ()
-
-
-let dm_bind0
-  (a b : Type)
-  (wp_v : hist a)
-  (wp_f:  a -> hist b)
-  (post_v: pure_post a)
-  (post_f: a -> pure_post b)
-  (v : dm a wp_v post_v)
-  (f : (x:a{post_v x} -> dm b (wp_f x) (bind_post post_v post_f))) :
-  Tot (dm b (hist_bind wp_v wp_f) (bind_post post_v post_f)) =
-  lemma_theta_is_monad_morphism_bind v f;
-  lemma_hist_monotonic a b wp_v wp_f post_v post_f v f;
-  io_bind v f
-  
 let dm_bind
   (a b : Type)
   (wp_v : hist a)
   (wp_f: a -> hist b)
-  (post_v: pure_post a)
-  (post_f: a -> pure_post b)
-  (v : dm a wp_v post_v)
-  (f : (x:a{post_v x} -> dm b (wp_f x) (post_f x))) :
-  Tot (dm b (hist_bind wp_v wp_f) (bind_post post_v post_f)) =
-  let f' : (x:a{post_v x} -> dm b (wp_f x) (bind_post post_v post_f)) = begin
-    fun x -> 
-      dm_subcomp (post_f x) (bind_post post_v post_f) (wp_f x) (wp_f x) (f x) _ _
-  end in
-  dm_bind0 a b wp_v wp_f post_v post_f v f'
+  (v : dm a wp_v)
+  (f : (x:a -> dm b (wp_f x))) :
+  Tot (dm b (hist_bind wp_v wp_f)) =
+  lemma_theta_is_monad_morphism_bind v f;
+  (** hist is monotonic.
+  
+  assert (theta (io_bind v f) == hist_bind (theta v) (fun x -> theta (f x)));
+  assert (wp_v `hist_ord` theta v);
+  assert (forall r. wp_f r `hist_ord` theta (f r));
+  assert (hist_bind wp_v wp_f `hist_ord` hist_bind (theta v) (fun x -> theta (f x)));
 
-////////////////////////////////////////////////////////////////////////////////////////
+  (** goal: **)
+  assert (hist_bind wp_v wp_f `hist_ord` theta (io_bind v f));**)
+  io_bind v f
 
-let l_repr (a:Type) (p:pure_pre) (q:pure_post a) (wp:hist a) = 
-  squash p -> dm a wp q
-
-let l_return (a:Type) (x:a) : l_repr a True (return_post x) (hist_return x) = fun () -> dm_return a x
-
-unfold let trivial_pre : pure_pre = True
-
-unfold
-let bind_pre (#a:Type) (p1:pure_pre) (q1:pure_post a) (p2:a -> pure_pre) : pure_pre
-  = p1 /\ (forall x. q1 x ==> p2 x)
-
-let l_bind (a b:Type)
-  (p1:pure_pre) (q1:pure_post a)
-  (p2:a -> pure_pre) (q2:a -> pure_post b)
-  (wp1:hist a) (wp2:a -> hist b)
-  (f:l_repr a p1 q1 wp1) (g:(x:a) -> l_repr b (p2 x) (q2 x) (wp2 x)) :
-  Tot (l_repr b (bind_pre p1 q1 p2) (bind_post q1 q2) (hist_bind wp1 wp2)) =
-  fun _ -> dm_bind a b wp1 wp2 q1 q2 (f _) (fun x -> g x _)
-
-let l_subcomp (a:Type) (p1 p2:pure_pre) (q1 q2:pure_post a) (wp1:hist a) (wp2:hist a) (f:l_repr a p1 q1 wp1)
-  : Pure (l_repr a p2 q2 wp2)
-    (requires (
-      (p2 ==> p1) /\
-      (forall x. q1 x ==> q2 x) /\
-      (wp1 `hist_ord` wp2)))
+let dm_subcomp (a:Type) (wp1 wp2: hist a) (f : dm a wp1) :
+  Pure (dm a wp2)
+    (requires hist_ord wp2 wp1)
     (ensures fun _ -> True) =
-  fun _ -> dm_subcomp q1 q2 wp1 wp2 (f _) _ _
+  f
 
-unfold
-let l_if_then_else 
-  (a : Type)
-  (p1 p2: pure_pre)
-  (q1 q2: pure_post a)
-  (wp1: hist a)
-  (wp2: hist a)
-  (f : l_repr a p1 q1 wp1)
-  (g : l_repr a p2 q2 wp2)
-  (b : bool) : Type =
-  l_repr a
-    ((b ==> p1) /\ ((~b) ==> p2)) 
-    (fun x -> (b ==> q1 x) /\ ((~b) ==> q2 x)) 
-    (hist_if_then_else wp1 wp2 b)
+let dm_if_then_else (a : Type) (wp1 wp2: hist a) (f : dm a wp1) (g : dm a wp2) (b : bool) : Type =
+  dm a (hist_if_then_else wp1 wp2 b)
 
-[@@allow_informative_binders]
 total
 reifiable
 reflectable
 layered_effect {
-  IOwp : a:Type -> p : pure_pre -> q : pure_post a -> wp : hist a -> Effect
+  IOwp : a:Type -> wp : hist a -> Effect
   with
-       repr       = l_repr 
-     ; return     = l_return
-     ; bind       = l_bind
+       repr       = dm 
+     ; return     = dm_return
+     ; bind       = dm_bind
 
-     ; subcomp      = l_subcomp
-     ; if_then_else = l_if_then_else
+     ; subcomp      = dm_subcomp
+     ; if_then_else = dm_if_then_else
 }
 
+let elim_pure #a #w (f : unit -> PURE a w) :
+  Pure a
+    (requires w (fun _ -> True))
+    (ensures fun r -> forall post. w post ==> post r) =
+  FStar.Monotonic.Pure.elim_pure_wp_monotonicity_forall ();
+  f ()
 
 (** inspired from fstar/examples/layeredeffects/Alg.fst **)
-let lift_pure_l (a : Type) (w : pure_wp a) (f:(eqtype_as_type unit -> PURE a w)) :
-  l_repr a (as_requires w) (as_ensures w) (wp_lift_pure_hist w) =
-  FStar.Monotonic.Pure.elim_pure_wp_monotonicity_forall ();
-  let r = f () in
-  let r'  = l_return a r in
-  l_subcomp a True (as_requires w) (fun x -> x == r) (as_ensures w) (hist_return r) (wp_lift_pure_hist w) r'
+let lift_pure_dm (a : Type) (w : pure_wp a) (f:(eqtype_as_type unit -> PURE a w)) :
+  Pure (dm a (wp_lift_pure_hist w)) (requires w (fun _ -> True)) (ensures fun _ -> True) =
+  let r = elim_pure #a #w f in
+  let r' : dm a (hist_return r) = dm_return a r in
+  dm_subcomp _ (hist_return r) (wp_lift_pure_hist w) r'
 
-sub_effect PURE ~> IOwp = lift_pure_l
+sub_effect PURE ~> IOwp = lift_pure_dm
 
 effect IO
   (a:Type)
   (pre : trace -> Type0)
   (post : trace -> trace -> a -> Type0) =
-  IOwp a 
-    True
-    (fun _ -> True)
-    (fun (p:hist_post a) (h:trace) -> pre h /\ (forall lt r. post h lt r ==> p lt r)) 
-
-assume val p' : prop
-assume val pure_lemma (_:unit) : Lemma p'
-assume val some_f : unit -> IO unit (requires (fun _ -> p')) (ensures fun _ _ _ -> True)
-  
-let test () : IO unit (fun _ -> True) (fun _ _ _ -> True) by (explode (); dump "H") =
-  pure_lemma ();
-  assert p'
-  
-let test' () : IO unit (fun _ -> True) (fun _ _ _ -> True) =
-  pure_lemma ();
-  some_f ()
-
-let test'' () : IO unit (fun _ -> True) (fun _ _ _ -> True) by (explode (); dump "H") =
-  pure_lemma ();
-  assert p';
-  some_f ()
+  IOwp a (fun (p:hist_post a) (h:trace) ->
+    pre h /\ (forall lt r. post h lt r ==>  p lt r))
 
 let static_cmd
   (cmd : io_cmds)
@@ -235,19 +144,16 @@ let static_cmd
     (requires (fun h -> io_pres cmd argz h))
     (ensures (fun h lt r ->
         lt == [convert_call_to_event cmd argz r])) =
-  IOwp?.reflect (fun _ -> io_call cmd argz)
+  IOwp?.reflect (io_call cmd argz)
 
-let testStatic2 () : IO unit (fun _ -> True) (fun _ _ _ -> True) by (
-    explode ();
-    dump "H")=
+let testStatic2 () : IO unit (fun _ -> True) (fun _ _ _ -> True) =
   let fd = static_cmd Openfile "../Makefile" in
-  if Some? fd then begin (** test if Openfile was successful **)
+  if Some? fd then (** test if Openfile was successful **)
     let msg = static_cmd Read (Some?.v fd) in
     let _ = static_cmd Close (Some?.v fd) in
     ()
-  end else ()
+  else ()
 
 let testStatic3 (fd:file_descr) : IO unit (fun h -> is_open fd h) (fun h lt r -> ~(is_open fd (trace_append h lt))) =
   let _ = static_cmd Close fd in
   ()
-
